@prefix : <http://aria.abdoulsy.eu/ontology/ADSP/Web_Project#> .
@prefix owl: <http://www.w3.org/2002/07/owl#> .
@prefix rdf: <http://www.w3.org/1999/02/22-rdf-syntax-ns#> .
@prefix xml: <http://www.w3.org/XML/1998/namespace> .
@prefix xsd: <http://www.w3.org/2001/XMLSchema#> .
@prefix rdfs: <http://www.w3.org/2000/01/rdf-schema#> .
@base <http://aria.abdoulsy.eu/ontology/ADSP/Web_Project> .

<http://aria.abdoulsy.eu/ontology/ADSP/Web_Project> rdf:type owl:Ontology ;
                                                    
                                                    owl:versionIRI <http://aria.abdoulsy.eu/ontology/ADSP/Web_Project/0.0.1> ;
                                                    
                                                    rdfs:comment "The Project Ontology under the ADSP (Application Development Surveillance Platform)"^^xsd:string .


#################################################################
#
#    Classes
#
#################################################################


###  http://aria.abdoulsy.eu/ontology/ADSP/Web_Project#Code_Versioning_System

:Code_Versioning_System rdf:type owl:Class .



###  http://aria.abdoulsy.eu/ontology/ADSP/Web_Project#Commit

:Commit rdf:type owl:Class ;
        
        rdfs:subClassOf :Code_Versioning_System ;
        
        rdfs:comment "A Commit on a versionning system is the way to save the current state of the entire project Files with a message annotation"^^xsd:string .



###  http://aria.abdoulsy.eu/ontology/ADSP/Web_Project#Commit_Hash

:Commit_Hash rdf:type owl:Class ;
             
             rdfs:subClassOf :Code_Versioning_System ;
             
             rdfs:comment "a Commit Hash is a MD5 hashed version of the current state of the project referencing the commit, usually only the first 5 or so characters are enough to retrieve the commit"^^xsd:string .



###  http://aria.abdoulsy.eu/ontology/ADSP/Web_Project#Commit_Message

:Commit_Message rdf:type owl:Class ;
                
                rdfs:subClassOf :Code_Versioning_System ;
                
                rdfs:comment "A Commit message is a message created or generated by the user to give an annotation on every saved version of the Project"^^xsd:string .



###  http://aria.abdoulsy.eu/ontology/ADSP/Web_Project#Directory

:Directory rdf:type owl:Class ;
           
           rdfs:comment "A Directory is a special File referencing other files, and their metadata"^^xsd:string .



###  http://aria.abdoulsy.eu/ontology/ADSP/Web_Project#File

:File rdf:type owl:Class ;
      
      rdfs:comment "A Document using the file:// protocol"^^xsd:string .



###  http://aria.abdoulsy.eu/ontology/ADSP/Web_Project#Git

:Git rdf:type owl:Class ;
     
     rdfs:subClassOf :Code_Versioning_System ;
     
     rdfs:comment "The Git Versioning system allows to create different retro-compatible versions of the code associated with a project"^^xsd:string .



###  http://aria.abdoulsy.eu/ontology/ADSP/Web_Project#Mac_OSX

:Mac_OSX rdf:type owl:Class .



###  http://aria.abdoulsy.eu/ontology/ADSP/Web_Project#OS_Path

:OS_Path rdf:type owl:Class ;
         
         rdfs:subClassOf :Operating_System ;
         
         rdfs:comment "a Path is a string locating a file or a directory in an Operating System"^^xsd:string .



###  http://aria.abdoulsy.eu/ontology/ADSP/Web_Project#Operating_System

:Operating_System rdf:type owl:Class .



###  http://aria.abdoulsy.eu/ontology/ADSP/Web_Project#Program

:Program rdf:type owl:Class ;
         
         rdfs:comment "a Program or Application, is a set of operations in an Operating System set to DO something"^^xsd:string .



###  http://aria.abdoulsy.eu/ontology/ADSP/Web_Project#Project

:Project rdf:type owl:Class ;
         
         rdfs:comment "The Concept of a Project"^^xsd:string .



###  http://aria.abdoulsy.eu/ontology/ADSP/Web_Project#Virtual_Machine

:Virtual_Machine rdf:type owl:Class .



###  http://aria.abdoulsy.eu/ontology/ADSP/Web_Project#Web_Project

:Web_Project rdf:type owl:Class ;
             
             rdfs:subClassOf :Project ;
             
             rdfs:comment "A project destined to be on a Web Server for internet use"^^xsd:string .




###  Generated by the OWL API (version 4.2.3.20160319-0906) https://github.com/owlcs/owlapi

